Spec/chapter-2.dfy
@@ -1,3 +1,5 @@
+// Book page: 71 
+
 // • p2.1  Write a program that displays the dimensions of a letter-size (8.5 × 11 inches) sheet 
 // of paper in millimeters. There are 25.4 millimeters per inch. 
 // Use constants and comments in your program.
